libs/ml/FFICallbacks.ml
@@ -1,0 +1,7 @@
+type cookie = int
+external ocaml_send_tcp2: cookie -> string -> int = "ocaml_send_tcp"
+external ocaml_recv_tcp2: cookie -> string -> int = "ocaml_recv_tcp"
+
+let ocaml_send_tcp cookie b = ocaml_send_tcp2 cookie b
+let ocaml_recv_tcp cookie b = ocaml_recv_tcp2 cookie b
+
