src/tls/FFICallbacks.mli
@@ -1,0 +1,4 @@
+type cookie = int
+val ocaml_send_tcp: cookie -> string -> int
+val ocaml_recv_tcp: cookie -> string -> int
+
