src/tls/mitlsffi.h
@@ -12,7 +12,6 @@ extern void * FFI_mitls_prepare_client_hello(/* in out */ size_t *state, /* out 
 extern int FFI_mitls_handle_server_hello(/* in out */ size_t *state, char* header, size_t header_size, char *record, size_t record_size);
 extern int FFI_mitls_handle_encrypted_extensions(/* in out */ size_t *state, char* header, size_t header_size, char *record, size_t record_size);
 extern int FFI_mitls_handle_certificate_verify12(/* in out */ size_t *state, char* header, size_t header_size, char *record, size_t record_size);
-extern int FFI_mitls_handle_certificate_verify13(/* in out */ size_t *state, char* header, size_t header_size, char *record, size_t record_size);
 extern int FFI_mitls_handle_server_key_exchange(/* in out */ size_t *state, char* header, size_t header_size, char *record, size_t record_size);
 extern int FFI_mitls_handle_server_hello_done(/* in out */ size_t *state, char* header, size_t header_size, char *record, size_t record_size);
 extern void * FFI_mitls_prepare_client_key_exchange(/* in out */ size_t *state, /* out */ size_t *packet_size); // Returns NULL for failure, or a TCP packet to be sent then freed with FFI_mitls_free_packet()
@@ -23,5 +22,19 @@ extern int FFI_mitls_handle_server_finished(/* in out */ size_t *state, char* he
 
 extern void * FFI_mitls_prepare_send(/* in out */ size_t *state, const void* buffer, size_t buffer_size, /* out */ size_t *packet_size); // Returns NULL for failure, or a TCP packet to be sent then freed with FFI_mitls_free_packet()
 extern void * FFI_mitls_handle_receive(/* in out */ size_t *state, char* header, size_t header_size, char *record, size_t record_size, /* out */ size_t *packet_size);     // Returns NULL for failure, a plaintext packet to be freed with FFI_mitls_free_packet()
+
+struct _FFI_mitls_callbacks;
+typedef int (*pfn_FFI_send)(struct _FFI_mitls_callbacks *callbacks, const void *buffer, size_t buffer_size);
+typedef int (*pfn_FFI_recv)(struct _FFI_mitls_callbacks *callbacks, void *buffer, size_t buffer_size);
+
+struct _FFI_mitls_callbacks {
+    pfn_FFI_send send;
+    pfn_FFI_recv recv;
+};
+
+extern int FFI_mitls_connect13(struct _FFI_mitls_callbacks *callbacks, /* out */ size_t *stateptr);
+extern void * FFI_mitls_prepare_send13(/* in out */ size_t *state, const void* buffer, size_t buffer_size, /* out */ size_t *packet_size); // Returns NULL for failure, or a TCP packet to be sent then freed with FFI_mitls_free_packet()
+extern void * FFI_mitls_handle_receive13(/* in out */ size_t *state, char* header, size_t header_size, char *record, size_t record_size, /* out */ size_t *packet_size);     // Returns NULL for failure, a plaintext packet to be freed with FFI_mitls_free_packet()
+
 
 #endif // HEADER_MITLS_FFI_H
