libs/ml/FFICallbacks.fst
@@ -1,0 +1,8 @@
+module FFICallbacks
+
+open Platform.Bytes
+
+type cookie = Prims.int
+
+assume val ocaml_send_tcp: cookie -> cbytes -> Tot int
+assume val ocaml_recv_tcp: cookie -> cbytes -> Tot int
